

CLI – Øvelsestimer

Øvelsestimer 1

Problem 1.1 Given the following sets $S = \{1; 2; 3; 6; 7; 9\}$ and $R = \{2; 4; 5; 6; 7\}$ state

a) $S \cup R$

- $\{1, 2, 3, 4, 5, 6, 7, 9\}$

b) $S \cap R$

- $\{2, 6, 7\}$

c) $S \setminus R$

- $\{1, 3, 9\}$

d) $R \setminus S$

- $\{4, 5\}$

e) $|S|$

- 6

f) $|R \setminus S|$

- 2

Problem 1.2 State these expression as simple rational numbers or fractions:

a) $\frac{7}{3} - \frac{1}{2}$

$$\frac{7 * 2}{3 * 2} - \frac{1 * 3}{2 * 3} =$$

$$\frac{14}{6} - \frac{3}{6} =$$

$$\frac{11}{6}$$

$$-\frac{a}{b} = \frac{-a}{b} = \frac{a}{-b}$$

$$\frac{a}{b} + \frac{c}{d} = \frac{a \cdot d + c \cdot b}{b \cdot d}$$

$$b) \pi + \frac{3}{5}$$

$$pi = 3,14$$

$$\frac{3}{5} = 0,6$$

$$3,14 + 0,6 = 3,74$$

$$a = \frac{a}{1}$$

$$\frac{a}{b} + \frac{c}{d} = \frac{a \cdot d + c \cdot d}{b \cdot d}$$

$$c) \frac{3x^2}{a} + 2x$$

$$a = \frac{1}{x}$$

$$\frac{3x^2}{a} + \frac{2x}{1} =$$

$$\frac{3x^2}{a} + \frac{a \cdot 2x}{a \cdot 1} =$$

$$\frac{3x^2}{a} + \frac{a \cdot 2x}{a} =$$

$$\frac{3x^2}{a} + \frac{2ax}{a} =$$

$$\frac{3x^2 + 2ax}{a}$$

$$a = \frac{a}{1}$$

$$\frac{a}{b} + \frac{c}{d} = \frac{a \cdot d + c \cdot d}{b \cdot d}$$

$$d) \frac{a}{4x^2} - \frac{x^2}{a}$$

$$\frac{a \cdot a}{4x^2 \cdot a} - \frac{4x^2 \cdot x^2}{4x^2 \cdot a} =$$

$$\frac{a^2}{4ax^2} - \frac{4x^4}{4ax^2} =$$

$$\frac{a^2 - 4x^4}{4ax^2}$$

$$-\frac{a}{b} = \frac{-a}{b} = \frac{a}{-b}$$

$$\frac{a}{b} + \frac{c}{d} = \frac{a \cdot d + c \cdot d}{b \cdot d}$$

$$a^2 - b^2 = (a + x)(a - x)$$

$$e) \frac{1}{\frac{a}{(x^2+1)}} - \frac{1}{a}$$

$$\begin{aligned} \frac{x^2+1}{a} - \frac{-1}{a} &= \\ \frac{x^2+1}{a} + \frac{-1}{a} &= \\ \frac{(x^2+1)a - 1 * a}{a * a} &= \\ \frac{a * x^2 + a - a}{a^2} &= \\ \frac{a * x^2}{a^2} &= \\ \frac{x^2}{a} \end{aligned}$$

$$\frac{1}{\frac{a}{b}} = \frac{b}{a}$$

$$-\frac{a}{b} = \frac{-a}{b} = \frac{a}{-b}$$

$$\frac{a}{b} + \frac{c}{d} = \frac{a \cdot d + c \cdot d}{b \cdot d}$$

$$a(b+c) = ab + ac$$

$$f) \frac{a}{2b+3a} - \frac{b}{a+1}$$

$$\begin{aligned} \frac{a}{2b+3a} + \frac{-b}{a+1} &= \\ \frac{a(a+1) - (2b+3a)b}{(2b+3a)(a+1)} &= \end{aligned}$$

$$-\frac{a}{b} = \frac{-a}{b} = \frac{a}{-b}$$

$$\frac{a}{b} + \frac{c}{d} = \frac{a \cdot d + c \cdot d}{b \cdot d}$$

Problem 1.3 Using the rules for exponentials simplify the following expressions:

$$a) 10^3 \cdot 5^{-2} \text{ (hint } 10 = 2 \cdot 5)$$

$$10^3 * 5^{-2} =$$

$$2^3 * 5^3 * \frac{1}{5^2} =$$

$$2^3 * 5^3 * \frac{1}{5^2} =$$

$$2^3 * 5 * 1 =$$

$$2^3 * 5 =$$

$$8 * 5 =$$

$$40$$

1. Since $10 = 2 \cdot 5$, we can substitute $10^3 \cdot 5^{-2} = (2 \cdot 5)^3 \cdot 5^{-2}$.
2. Using the rule $(a \cdot b)^n = a^n \cdot b^n$ we get $(2 \cdot 5)^3 \cdot 5^{-2} = 2^3 \cdot 5^3 \cdot 5^{-2}$.
3. Using the rule $a^n \cdot a^m = a^{n+m}$ we get $2^3 \cdot 5^3 \cdot 5^{-2} = 2^3 \cdot 5^{3-2} = 2^3 \cdot 5$.

b) $\frac{3^5}{3^2}$

$$\frac{3^5}{3^2} =$$

$$3^{5-2} =$$

$$3^3$$

1. Using the rule $\frac{a^n}{a^m} = a^{n-m}$ we get $\frac{3^5}{3^2} = 3^{5-2} = 3^3$

c) $5 \cdot 25^8$ (hint $25 = 5^2$)

$$5 * (5^2)^8 =$$

$$5 * 5^{2*8} =$$

$$5 * 5^{16} =$$

$$5^1 * 5^{16} =$$

$$5^{17}$$

1. Since $25 = 5^2$, we can substitute to get $5 \cdot 25^8 = 5 \cdot (5^2)^8$
2. Using the rule $(a^n)^m = a^{n \cdot m}$ we get $5 \cdot (5^2)^8 = 5 \cdot 5^{2 \cdot 8} = 5 \cdot 5^{16}$
3. Using the rule $a^n \cdot a^m = a^{n+m}$ we get $5 \cdot 5^{16} = 5^{17}$

d) $2^3 \sqrt[5]{6^{10}}$ (hint $6 = 3 \cdot 2$)

$$2^3 * 6^{\frac{10}{5}} =$$

$$2^3 * 6^{\frac{10/5}{5}} =$$

$$2^3 * 6^{\frac{2}{1}} =$$

$$2^3 * 6^2 =$$

$$2^3 * (2 * 3)^2 =$$

$$2^3 * 2^2 * 3^2 =$$

$$2^5 * 3^2$$

1. Using the rule $\sqrt[n]{a^m} = a^{\frac{m}{n}}$ we get $2^3 \sqrt[5]{6^{10}} = 2^3 \cdot 6^{\frac{10}{5}} = 2^3 \cdot 6^2$
2. Since $6 = 3 \cdot 2$ we can substitute $2^3 \cdot 6^2 = 2^3 \cdot (3 \cdot 2)^2$
3. Using the rule $(a \cdot b)^n = a^n \cdot b^n$ we get $2^3 \cdot (3 \cdot 2)^2 = 2^3 \cdot 3^2 \cdot 2^2$
4. Using the rule $a^n \cdot a^m = a^{n+m}$ we get $2^3 \cdot 3^2 \cdot 2^2 = 2^{3+2} \cdot 3^2 = 2^5 \cdot 3^2$

e) $\sqrt[3]{7^{-21}}$

$$7^{\frac{-21}{3}} =$$

$$7^{\frac{-7}{1}} =$$

$$7^{-7} =$$

$$\frac{1}{7^7}$$

1. Using the rule $\sqrt[n]{a^m} = a^{\frac{m}{n}}$ we get $\sqrt[3]{7^{-21}} = 7^{-\frac{21}{3}} = 7^{-7}$
2. Using the rule $a^{-n} = \frac{1}{a^n}$ we get $7^{-7} = \frac{1}{7^7}$

f) $\sqrt[4]{(2^2)^5}$

$$\begin{aligned}\sqrt[4]{2^{2 \cdot 5}} &= & 1. \text{ Using the rule } (a^n)^m &= a^{n \cdot m} \text{ we get } \sqrt[4]{(2^2)^5} = \sqrt[4]{2^{2 \cdot 5}} = \sqrt[4]{2^{10}} \\ \sqrt[4]{2^{10}} &= & 2. \text{ Using the rule } \sqrt[n]{a^m} &= a^{\frac{m}{n}} \text{ we get } \sqrt[4]{2^{10}} = 2^{\frac{10}{4}} = 2^{\frac{5}{2}} \\ 2^{\frac{10}{4}} &= \\ 2^{\frac{5}{2}} &= \end{aligned}$$

Problem 1.4 Write the following inequalities as intervals of the real line

a) $x \leq 100$

Numbers smaller or equal than 100: $(-\infty; 100]$

b) $x > 0$ and $x < 10$

Numbers between 0 and 10 (not included) $(0; 10)$

c) $x \geq -10$ and $x < 5$

Numbers larger or equal than -10 and smaller than 5: $[-10; 5)$

d) $x \geq -1$

Numbers larger or equal than -1: $[-1, \infty)$

e) $x < -5$ or $x \geq 5$

Numbers smaller than -5 or larger than 5: $(-\infty; -5) \cup [5; \infty)$

f) $x \neq 3$

Numbers different than 3: $(-\infty, \infty) \setminus \{3\}$ or $(-\infty, 3) \cup (3, \infty)$

Problem 1.5 Solve the following inequalities for x:

a) $6x - 5 > 7$

$$6x - 5 + 5 > 7 + 5 =$$

$$6x > 12 =$$

$$\frac{6}{6} * x > \frac{12}{6} =$$

$$x > 2 \ (2, \infty)$$

b) $-2x \geq 4$

$$-\frac{2x}{-2} < \frac{4}{-2} =$$

$$x > -2(-\infty; -2)$$

c) $5x - 3 < 7 - 3x$

$$5x - 3 + 3 < 7 + 3 - 3x =$$

$$5x < 10 - 3x =$$

$$5x + 3x < 10 - 3x + 3x =$$

$$8x < 10 =$$

$$\frac{8x}{8} < \frac{10}{8} =$$

$$x = \frac{\frac{10}{8}}{8} =$$

$$x = \frac{5}{4}$$

d) $\frac{6-x}{-4} \geq \frac{3x-4}{2}$

$$4 * \frac{6-x}{-4} > 4 * \frac{3x-4}{2} =$$

$$-(6-x) > 2 * (3x-4) =$$

$$-6+x > 6x-8 =$$

$$-6+6+x-6x > -8+6 =$$

$$x-6x > -2 =$$

$$5x > -2 =$$

$$\frac{-5x}{-5} > \frac{-2}{-5} =$$

$$x = \frac{2}{5}$$

Kommenterede [BK1]: Ethvert negativt tal delt med et negativt giver et positivt tal

e) $\frac{1}{x} > 6$

$$\begin{aligned}\frac{1}{x} - 6 &> \textcolor{red}{6} - \textcolor{red}{6} = \\ \frac{1-6}{x} &> 0 = \\ 1-6x &> 0 = \\ \textcolor{red}{-1} + \textcolor{red}{1} - 6x &> -1 = \\ -6x &> -1 = \\ -\frac{6}{-6} * x &> -\frac{1}{-6} = \\ x &> \frac{1}{6} \quad (0, \frac{1}{6})\end{aligned}$$

f) $\frac{x+1}{x-1} \geq 2$

f) $\frac{x+1}{x-1} \geq 2$ we can multiply both sides by $x-1$ but since $x-1$ can be negative we need to account for the change of sign of the inequality.

- $x-1 > 0$, i.e. $x > 1$, leads to $(x-1)\frac{x+1}{x-1} = x+1 \geq 2(x-1) = 2x-2$, and adding $2-x$ on both sides leads to $x+1+2-x = 3 \geq 2x-2+2-x = x$, i.e. $3 \geq x$. Both inequalities must hold simultaneously $x > 1$ and $x \leq 3$, which leads to the solution $1 < x \leq 3$.
- $x-1 < 0$, i.e. $x < 1$, leads to $(x-1)\frac{x+1}{x-1} = x+1 \leq 2(x-1) = 2x-2$ (change of inequality sign), which by adding leads to $2-x$ on both sides leads to $x+1+2-x = 3 \leq 2x-2+2-x = x$, i.e. $x \geq 3$. Both conditions cannot hold simultaneously and therefore $x-1 < 0$ does not lead to a valid solution.

$$g) \frac{x}{2-x} < 0$$

g) $\frac{x}{2-x} < 0$. We can multiply both sides by $2-x$ but since $2-x$ can be negative we need to account for the change on the sign of the inequality.

- If $2-x > 0$ (i.e. $x < 2$) we get $x < 0$ (i.e. no sign change). Since both inequalities ($x < 0$ and $x < 2$) must be fulfilled simultaneously, the numbers which fulfil both are $x < 0$ (the most restrictive).
- If $2-x < 0$ (i.e. $x > 2$) we get $x > 0$ (i.e. sign change after multiplication). Since both inequalities ($x > 0$ and $x > 2$) must be fulfilled simultaneously, the numbers which fulfil both are $x > 2$ (the most restrictive).

If $2-x > 0$ we get $x < 0$, and if $2-x < 0$ we get $x > 2$, therefore the solution is $x < 0$ or $x > 2$, which as interval can be written as $(-\infty, 0) \cup (2, \infty)$

Alternative solution: (Using function notation that we will see later in the course) There is an alternative way of solving inequalities of the form $\frac{f(x)}{g(x)} > 0$, $\frac{f(x)}{g(x)} < 0$, $\frac{f(x)}{g(x)} \geq 0$ and $\frac{f(x)}{g(x)} \leq 0$ (or any you can convert to this form). In this case, since $\frac{x}{2-x} < 0$, that happens when: ($x < 0$ and $2-x > 0$) or ($x > 0$ and $2-x < 0$). This leads to the combination of two solutions:

- $x < 0$ and $2-x > 0$ (i.e. $x < 2$). In this case, the numbers which are both smaller than zero ($x < 0$) and simultaneously smaller than two ($x < 2$) are only those smaller than zero, i.e. $x < 0$ which as an interval is $(-\infty, 0)$
- $x > 0$ and $2-x < 0$ (i.e. $x > 2$). In this case, the numbers which are bigger than zero ($x > 0$) and simultaneously bigger than two ($x > 2$) are those bigger than two, i.e. $x > 2$, which as an interval is $(2, \infty)$.

Since one or the other condition must hold the result is $(-\infty, 0) \cup (2, \infty)$, which is the same as for the solution above.

$$h) \frac{x^2-1}{x-3} \geq 0$$

h) $\frac{x^2-1}{x-3} \geq 0$. We can multiply both sides by $x-3$ but since $x-3$ can be negative we need to account for the change on the sign of the inequality.

- If $x-3 > 0$ (i.e. $x > 3$) we get $x^2-1 \geq 0$ (i.e. no sign change), which leads to $x^2 \geq 1$, and this occurs when $x \geq 1$ or $x \leq -1$. There is no number x bigger than three ($x > 3$) which is simultaneously smaller than negative one ($x \leq -1$), therefore these conditions do not lead to a valid solution. On the other hand, $x \geq 1$ and $x > 3$ have to be fulfilled simultaneously, and that happens for any $x > 3$.

- If $x - 3 < 0$ (i.e. $x < 3$) we get $x^2 - 1 \leq 0$ (i.e. sign change after multiplication), which leads to $x^2 \leq 1$, and this occurs when $-1 \leq x \leq 1$. Since all the numbers between negative one and one are smaller than three, the resulting condition is $-1 \leq x \leq 1$

If $x - 3 > 0$ we get $x > 3$, and if $x - 3 < 0$ we get $-1 \leq x \leq 1$, therefore the solution as interval can be written as $[-1, 1] \cup (3, \infty)$

Alternative solution: Since $\frac{x^2-1}{x-3} \geq 0$, that happens when: $(x^2 - 1 \geq 0 \text{ and } x - 3 > 0)$ or $(x^2 - 1 \leq 0 \text{ and } x - 3 < 0)$. Note that the denominator $x - 3$ cannot be zero, but the numerator $x^2 - 1$ can since we have equality (\geq) sign, so we use equality in the numerator and strict inequality in the denominator. This leads to the combination of two solutions:

- $x^2 - 1 \geq 0$ (i.e. $x^2 \geq 1$) **and** $x - 3 > 0$ (i.e. $x > 3$). Like in the previous solution we get that these two conditions are fulfilled simultaneously when $x > 3$.
- $x^2 - 1 \leq 0$ (i.e. $x^2 \leq 1$) **and** $x - 3 < 0$ (i.e. $x < 3$). Like in the previous solution we get that these conditions are fulfilled simultaneously when $-1 \leq x \leq 1$.

Since one or the other condition must hold the result is $[-1, 1] \cup (3, \infty)$, which is the same as for the solution above.